coq_translation/default/examples/ink_contracts/Proofs/erc20.v
@@ -4,18 +4,14 @@ Require CoqOfRust.examples.ink_contracts.Simulations.erc20.
 Require CoqOfRust.examples.ink_contracts.erc20.
 
 Module State.
-  Module State.
-    (** The state is a single cell containing the contract's state. This is an
-        option type as it may or may not be allocated. *)
-    Definition t : Set := option erc20.Erc20.t.
-  End State.
+  Definition t : Set := option erc20.Erc20.t.
+End State.
 
-  Module Address.
-    (** As there is a single cell in the state, the address type carries no
-        information. *)
-    Definition t : Set := unit.
-  End Address.
+Module Address.
+  Definition t : Set := unit.
+End Address.
 
+Module StateInstance.
   Global Instance I : State.Trait State.t Address.t := {
     State.get_Set address :=
       match address with
@@ -27,7 +23,7 @@ Module State.
       end;
     State.alloc_write address state value :=
       match address, value with
-      | tt, _ => Some (Some value)
+      | tt, value => Some (Some value)
       end;
   }.
 
@@ -35,29 +31,29 @@ Module State.
   Proof.
     sauto lq: on rew: off.
   Qed.
-End State.
+End StateInstance.
 
 Ltac run_symbolic_state_read :=
   match goal with
-  | |- Run.t (LowM.CallPrimitive (Primitive.StateRead ?address)) _ _ _ =>
+  | |- Run.t _ (LowM.CallPrimitive (Primitive.StateRead ?address)) _ _ _ =>
     let H := fresh "H" in
-    pose proof (H := Run.CallPrimitiveStateRead address);
+    epose proof (H := Run.CallPrimitiveStateRead _ address);
     apply H; reflexivity;
     clear H
   end.
 
 Ltac run_symbolic_state_write :=
   match goal with
-  | |- Run.t (LowM.CallPrimitive (Primitive.StateWrite ?address ?value)) _ _ _ =>
+  | |- Run.t _ (LowM.CallPrimitive (Primitive.StateWrite ?address ?value)) _ _ _ =>
     let H := fresh "H" in
-    pose proof (H := Run.CallPrimitiveStateWrite address value);
+    epose proof (H := Run.CallPrimitiveStateWrite _ address value);
     apply H; reflexivity;
     clear H
   end.
 
 Ltac run_symbolic_one_step :=
   match goal with
-  | |- Run.t _ _ _ _ =>
+  | |- Run.t _ _ _ _ _ =>
     econstructor ||
     run_symbolic_state_read ||
     run_symbolic_state_write
@@ -65,40 +61,6 @@ Ltac run_symbolic_one_step :=
 
 Ltac run_symbolic :=
   repeat run_symbolic_one_step.
-
-(** Starting from a state with a given [balance] for a given [owner], when we
-    read that information we get the expected [balance]. *)
-Lemma run_balance_of_impl'
-  (owner : erc20.AccountId.t)
-  (balance : Z)
-  fuel :
-  (* An initial state *)
-  let state := Some ({|
-    erc20.Erc20.total_supply := 0;
-    erc20.Erc20.balances := Lib.Mapping.insert owner balance Lib.Mapping.empty;
-    erc20.Erc20.allowances := Lib.Mapping.empty;
-  |}) in
-  (* The value [self] is allocated in the state *)
-  let self : M.Val (ref erc20.Erc20.t) := Ref.Imm (Ref.mut_ref tt) in
-  (* The value [owner] is an immediate value *)
-  let owner : M.Val (ref erc20.AccountId.t) := Ref.Imm (Ref.Imm owner) in
-  Run.t
-    (erc20.Impl_erc20_Erc20_t_2.balance_of_impl self owner fuel)
-    state
-    (* expected output *)
-    (inl (Ref.Imm balance))
-    (* the state does not change *)
-    state.
-Proof.
-  unfold erc20.Impl_erc20_Erc20_t_2.balance_of_impl.
-  run_symbolic.
-  { simpl.
-    rewrite Lib.Mapping.get_insert_eq.
-    run_symbolic.
-  }
-  { run_symbolic. }
-  { run_symbolic. }
-Qed.
 
 Module ReadMessage.
   (** A message that only read the store. *)
@@ -110,7 +72,7 @@ Module ReadMessage.
   .
 
   Definition dispatch {A : Set} (message : t A) : M (M.Val A) :=
-    let self : M.Val (ref erc20.Erc20.t) := Ref.Imm (Ref.mut_ref tt) in
+    let self := Ref.Imm (Ref.mut_ref tt) in
     match message with
     | total_supply => erc20.Impl_erc20_Erc20_t_2.total_supply self
     | balance_of owner =>
@@ -136,7 +98,7 @@ Module WriteMessage.
   .
 
   Definition dispatch (message : t) : M (M.Val ltac:(erc20.Result unit)) :=
-    let self : M.Val (ref erc20.Erc20.t) := Ref.Imm (Ref.mut_ref tt) in
+    let self := Ref.Imm (Ref.mut_ref tt) in
     match message with
     | transfer to value =>
       erc20.Impl_erc20_Erc20_t_2.transfer
@@ -158,10 +120,14 @@ Module WriteMessage.
 End WriteMessage.
 
 (** The simulation [total_supply] is valid. *)
-Lemma run_total_supply (storage : erc20.Erc20.t) fuel :
+Lemma run_total_supply
+    (env : erc20.Env.t)
+    (storage : erc20.Erc20.t)
+    fuel :
   let state := Some storage in
-  let self : M.Val (ref erc20.Erc20.t) := Ref.Imm (Ref.mut_ref tt) in
+  let self := Ref.Imm (Ref.mut_ref tt) in
   Run.t
+    env
     (erc20.Impl_erc20_Erc20_t_2.total_supply self fuel)
     state
     (inl (Ref.Imm (Simulations.erc20.total_supply storage)))
@@ -173,13 +139,15 @@ Qed.
 
 (** The simulation [balance_of] is valid. *)
 Lemma run_balance_of_impl
-  (storage : erc20.Erc20.t)
-  (owner : erc20.AccountId.t)
-  fuel :
+    (env : erc20.Env.t)
+    (storage : erc20.Erc20.t)
+    (owner : erc20.AccountId.t)
+    fuel :
   let state := Some storage in
-  let self : M.Val (ref erc20.Erc20.t) := Ref.Imm (Ref.mut_ref tt) in
+  let self := Ref.Imm (Ref.mut_ref tt) in
   let val_owner : M.Val (ref erc20.AccountId.t) := Ref.Imm (Ref.Imm owner) in
   Run.t
+    env
     (erc20.Impl_erc20_Erc20_t_2.balance_of_impl self val_owner fuel)
     state
     (inl (Ref.Imm (Simulations.erc20.balance_of_impl storage owner)))
@@ -197,13 +165,15 @@ Qed.
 
 (** The simulation [balance_of] is valid. *)
 Lemma run_balance_of
-  (storage : erc20.Erc20.t)
-  (owner : erc20.AccountId.t)
-  fuel :
+    (env : erc20.Env.t)
+    (storage : erc20.Erc20.t)
+    (owner : erc20.AccountId.t)
+    fuel :
   let state := Some storage in
-  let self : M.Val (ref erc20.Erc20.t) := Ref.Imm (Ref.mut_ref tt) in
+  let self := Ref.Imm (Ref.mut_ref tt) in
   let val_owner : M.Val erc20.AccountId.t := Ref.Imm owner in
   Run.t
+    env
     (erc20.Impl_erc20_Erc20_t_2.balance_of self val_owner fuel)
     state
     (inl (Ref.Imm (Simulations.erc20.balance_of storage owner)))
@@ -219,15 +189,17 @@ Qed.
 
 (** The simulation [allowance_impl] is valid. *)
 Lemma run_allowance_impl
-  (storage : erc20.Erc20.t)
-  (owner : erc20.AccountId.t)
-  (spender : erc20.AccountId.t)
-  fuel :
+    (env : erc20.Env.t)
+    (storage : erc20.Erc20.t)
+    (owner : erc20.AccountId.t)
+    (spender : erc20.AccountId.t)
+    fuel :
   let state := Some storage in
-  let self : M.Val (ref erc20.Erc20.t) := Ref.Imm (Ref.mut_ref tt) in
+  let self := Ref.Imm (Ref.mut_ref tt) in
   let val_owner : M.Val (ref erc20.AccountId.t) := Ref.Imm (Ref.Imm owner) in
   let val_spender : M.Val (ref erc20.AccountId.t) := Ref.Imm (Ref.Imm spender) in
   Run.t
+    env
     (erc20.Impl_erc20_Erc20_t_2.allowance_impl self val_owner val_spender fuel)
     state
     (inl (Ref.Imm (Simulations.erc20.allowance_impl storage owner spender)))
@@ -246,15 +218,17 @@ Qed.
 
 (** The simulation [allowance] is valid. *)
 Lemma run_allowance
-  (storage : erc20.Erc20.t)
-  (owner : erc20.AccountId.t)
-  (spender : erc20.AccountId.t)
-  fuel :
+    (env : erc20.Env.t)
+    (storage : erc20.Erc20.t)
+    (owner : erc20.AccountId.t)
+    (spender : erc20.AccountId.t)
+    fuel :
   let state := Some storage in
-  let self : M.Val (ref erc20.Erc20.t) := Ref.Imm (Ref.mut_ref tt) in
+  let self := Ref.Imm (Ref.mut_ref tt) in
   let val_owner : M.Val erc20.AccountId.t := Ref.Imm owner in
   let val_spender : M.Val erc20.AccountId.t := Ref.Imm spender in
   Run.t
+    env
     (erc20.Impl_erc20_Erc20_t_2.allowance self val_owner val_spender fuel)
     state
     (inl (Ref.Imm (Simulations.erc20.allowance storage owner spender)))
@@ -270,20 +244,22 @@ Qed.
 
 (** There are no panics with read messages. *)
 Lemma read_message_no_panic
-  (message : ReadMessage.t ltac:(erc20.Balance))
-  (storage : erc20.Erc20.t)
-  fuel :
-  let state := Some storage in
-  exists result,
-  Run.t
-    (ReadMessage.dispatch message fuel)
-    state
-    (* no errors in the result *)
-    (inl result)
-    (* the state does not change *)
-    state.
+    (env : erc20.Env.t)
+    (message : ReadMessage.t ltac:(erc20.Balance))
+    (storage : erc20.Erc20.t)
+    fuel :
+    let state := Some storage in
+    exists result,
+    Run.t
+      env
+      (ReadMessage.dispatch message fuel)
+      state
+      (* no errors in the result *)
+      (inl result)
+      (* the state does not change *)
+      state.
 Proof.
-  destruct message.
+  destruct message; simpl.
   { eexists.
     apply run_total_supply.
   }
@@ -295,24 +271,27 @@ Proof.
   }
 Qed.
 
+(** The simulation [transfer_from_to] is valid. *)
 Lemma run_transfer_from_to
-  (storage : erc20.Erc20.t)
-  (from : erc20.AccountId.t)
-  (to : erc20.AccountId.t)
-  (value : ltac:(erc20.Balance))
-  fuel :
-  let state := Some storage in
-  let self : M.Val (ref erc20.Erc20.t) := Ref.Imm (Ref.mut_ref tt) in
-  let val_from : M.Val (ref erc20.AccountId.t) := Ref.Imm (Ref.Imm from) in
-  let val_to : M.Val (ref erc20.AccountId.t) := Ref.Imm (Ref.Imm to) in
-  let val_value : M.Val ltac:(erc20.Balance) := Ref.Imm value in
-  let '(result, state') :=
-    Simulations.erc20.transfer_from_to storage from to value in
-  Run.t
-    (erc20.Impl_erc20_Erc20_t_2.transfer_from_to self val_from val_to val_value fuel)
-    state
-    (inl (Ref.Imm result))
-    (Some state').
+    (env : erc20.Env.t)
+    (storage : erc20.Erc20.t)
+    (from : erc20.AccountId.t)
+    (to : erc20.AccountId.t)
+    (value : ltac:(erc20.Balance))
+    fuel :
+    let state := Some storage in
+    let self := Ref.Imm (Ref.mut_ref tt) in
+    let val_from : M.Val (ref erc20.AccountId.t) := Ref.Imm (Ref.Imm from) in
+    let val_to : M.Val (ref erc20.AccountId.t) := Ref.Imm (Ref.Imm to) in
+    let val_value : M.Val ltac:(erc20.Balance) := Ref.Imm value in
+    let simulation :=
+      Simulations.erc20.transfer_from_to storage from to value in
+    Run.t
+      env
+      (erc20.Impl_erc20_Erc20_t_2.transfer_from_to self val_from val_to val_value fuel)
+      state
+      (inl (Ref.Imm (fst simulation)))
+      (Some (snd simulation)).
 Proof.
   unfold erc20.Impl_erc20_Erc20_t_2.transfer_from_to,
     Simulations.erc20.transfer_from_to.
@@ -324,4 +303,133 @@ Proof.
       rewrite H_lt ||
       apply run_balance_of_impl
     ).
+Qed.
+
+(** The simulation [transfer] is valid. *)
+Lemma run_transfer
+    (env : erc20.Env.t)
+    (storage : erc20.Erc20.t)
+    (to : erc20.AccountId.t)
+    (value : ltac:(erc20.Balance))
+    fuel :
+    let state := Some storage in
+    let self := Ref.Imm (Ref.mut_ref tt) in
+    let val_to : M.Val erc20.AccountId.t := Ref.Imm to in
+    let val_value : M.Val ltac:(erc20.Balance) := Ref.Imm value in
+    let simulation :=
+      Simulations.erc20.transfer env storage to value in
+    Run.t
+      env
+      (erc20.Impl_erc20_Erc20_t_2.transfer self val_to val_value fuel)
+      state
+      (inl (Ref.Imm (fst simulation)))
+      (Some (snd simulation)).
+Proof.
+  unfold erc20.Impl_erc20_Erc20_t_2.transfer,
+    Simulations.erc20.transfer.
+  with_strategy opaque [erc20.Impl_erc20_Erc20_t_2.transfer_from_to]
+    run_symbolic.
+  apply run_transfer_from_to.
+  all: run_symbolic.
+Qed.
+
+(** The simulation [approve] is valid. *)
+Lemma run_approve
+    (env : erc20.Env.t)
+    (storage : erc20.Erc20.t)
+    (spender : erc20.AccountId.t)
+    (value : ltac:(erc20.Balance))
+    fuel :
+    let state := Some storage in
+    let self := Ref.Imm (Ref.mut_ref tt) in
+    let val_spender : M.Val erc20.AccountId.t := Ref.Imm spender in
+    let val_value : M.Val ltac:(erc20.Balance) := Ref.Imm value in
+    let simulation :=
+      Simulations.erc20.approve env storage spender value in
+    Run.t
+      env
+      (erc20.Impl_erc20_Erc20_t_2.approve self val_spender val_value fuel)
+      state
+      (inl (Ref.Imm (fst simulation)))
+      (Some (snd simulation)).
+Proof.
+  unfold erc20.Impl_erc20_Erc20_t_2.approve,
+    Simulations.erc20.approve.
+  repeat (simpl || run_symbolic).
+Qed.
+
+(** The simulation [transfer_from] is valid. *)
+Lemma run_transfer_from
+    (env : erc20.Env.t)
+    (storage : erc20.Erc20.t)
+    (from : erc20.AccountId.t)
+    (to : erc20.AccountId.t)
+    (value : ltac:(erc20.Balance))
+    fuel :
+    let state := Some storage in
+    let self := Ref.Imm (Ref.mut_ref tt) in
+    let val_from : M.Val erc20.AccountId.t := Ref.Imm from in
+    let val_to : M.Val erc20.AccountId.t := Ref.Imm to in
+    let val_value : M.Val ltac:(erc20.Balance) := Ref.Imm value in
+    let simulation :=
+      Simulations.erc20.transfer_from env storage from to value in
+    Run.t
+      env
+      (erc20.Impl_erc20_Erc20_t_2.transfer_from self val_from val_to val_value fuel)
+      state
+      (inl (Ref.Imm (fst simulation)))
+      (Some (snd simulation)).
+Proof.
+  unfold erc20.Impl_erc20_Erc20_t_2.transfer_from,
+    Simulations.erc20.transfer_from.
+  destruct erc20.transfer_from_to as [result storage'] eqn:H_from_to.
+  destruct result as [[]|] eqn:H_result;
+    destruct (_ <? _) eqn:H_lt;
+    repeat (
+      simpl ||
+      with_strategy opaque [
+          erc20.Impl_erc20_Erc20_t_2.allowance_impl
+          erc20.Impl_erc20_Erc20_t_2.transfer_from_to
+        ]
+        run_symbolic ||
+      apply run_allowance_impl ||
+      apply run_transfer_from_to ||
+      rewrite H_lt ||
+      rewrite H_from_to
+    ).
+Qed.
+
+(** Starting from a state with a given [balance] for a given [owner], when we
+    read that information we get the expected [balance]. *)
+Lemma balance_of_impl_read_id
+  (env : erc20.Env.t)
+  (owner : erc20.AccountId.t)
+  (balance : Z)
+  fuel :
+  let storage := {|
+    erc20.Erc20.total_supply := 0;
+    erc20.Erc20.balances := Lib.Mapping.insert owner balance Lib.Mapping.empty;
+    erc20.Erc20.allowances := Lib.Mapping.empty;
+  |} in
+  (* An initial state *)
+  let state := Some storage in
+  (* The value [self] is allocated in the state *)
+  let self : M.Val (ref erc20.Erc20.t) := Ref.Imm (Ref.mut_ref tt) in
+  (* The value [owner] is an immediate value *)
+  let owner : M.Val (ref erc20.AccountId.t) := Ref.Imm (Ref.Imm owner) in
+  Run.t
+    env
+    (erc20.Impl_erc20_Erc20_t_2.balance_of_impl self owner fuel)
+    state
+    (* expected output *)
+    (inl (Ref.Imm balance))
+    (* the state does not change *)
+    state.
+Proof.
+  intros.
+  replace balance with (erc20.balance_of_impl storage owner).
+  apply run_balance_of_impl.
+  unfold erc20.balance_of_impl.
+  simpl.
+  now rewrite Lib.Mapping.get_insert_eq.
 Qed.
